Prove counter updates, modulo a lemma that's TBP

vale/code/crypto/aes/AES_helpers.fsti
@@ -131,3 +131,13 @@ val finish_cipher_opt (alg:algorithm) (input plain:quad32) (round_keys:seq quad3
             let state = quad32_xor state (quad32_xor plain (index round_keys (nr alg))) in
             state == quad32_xor plain (cipher_opaque alg input round_keys)))
 *)
+
+let lemma_incr_msb (orig ctr ctr':quad32) (increment:nat) : Lemma
+  (requires increment < 6 /\
+            ctr == reverse_bytes_quad32 orig /\
+            ctr.hi3 + (increment * 0x10000000) < pow2_32 /\
+            ctr' == Arch.Types.add_wrap_quad32 ctr (Mkfour 0 0 0 (increment * 0x10000000)))
+  (ensures  ctr' == reverse_bytes_quad32 (GCTR_s.inc32 orig increment))
+  =
+  admit()
+          
